LLVM_DS_RBT.thy
@@ -2,13 +2,12 @@ theory LLVM_DS_RBT
   imports
   "LLVM_DS_RBT/Free"
   "LLVM_DS_RBT/Insert/Insert"
-  "LLVM_DS_RBT/Insert/Naive_Insert"
   "LLVM_DS_RBT/Lookup/Lookup"
   "LLVM_DS_RBT/Lookup/Update"
- 
+
+  "LLVM_DS_RBT/Load_Store_Example"
   "LLVM_DS_RBT/Example/Export"
   "LLVM_DS_RBT/Bench_Export"
 begin
-
 
 end
