LLVM_DS_RBT/Assertion_Tree_Lookup.thy
@@ -1,0 +1,169 @@
+theory Assertion_Tree_Lookup
+  imports Extended_Assertion
+begin
+
+context rbt_impl
+begin
+
+fun p_node_of_key :: "_ \<Rightarrow> ('ki, 'vi) rbti \<Rightarrow> 'k  \<Rightarrow> _ option" where
+  "p_node_of_key ATEmpty _  _ = None"
+| "p_node_of_key br p kn =
+  (
+    if kn < (assn_tree.key br) then p_node_of_key (assn_tree.left br) (assn_tree.ll_left br) kn
+    else if kn > (assn_tree.key br) then p_node_of_key (assn_tree.right br) (assn_tree.ll_right br) kn
+    else Some (p, br)
+  )
+"
+
+fun ptr_of_key :: "_ \<Rightarrow> ('ki, 'vi) rbti \<Rightarrow> 'k  \<Rightarrow> ('ki, 'vi) rbti option" where
+  "ptr_of_key t ti k = map_option fst (p_node_of_key t ti k)"
+
+
+fun at_ptr_graph where
+  "at_ptr_graph ATEmpty _ = {}"
+| "at_ptr_graph (ATBranch c k v ci li ki vi ri al ar) p = 
+    {(k, p)} \<union> (at_ptr_graph al li) \<union> (at_ptr_graph ar ri)
+  "
+
+lemma ptr_of_key_less_none:
+  "rbt_of t |\<guillemotleft> k \<Longrightarrow> ptr_of_key t p k = None"
+  apply (induction t arbitrary: p)
+  by auto
+
+lemma p_node_of_key_less_none:
+  "rbt_of t |\<guillemotleft> k \<Longrightarrow> p_node_of_key t p k = None"
+  apply (induction t arbitrary: p)
+  by auto
+
+
+lemma ptr_of_key_greater_none:
+  "k \<guillemotleft>| rbt_of t \<Longrightarrow> ptr_of_key t p k = None"
+  apply (induction t arbitrary: p)
+  by auto
+
+
+lemma p_node_of_key_greater_none:
+  "k \<guillemotleft>| rbt_of t \<Longrightarrow> p_node_of_key t p k = None"
+  apply (induction t arbitrary: p)
+  by auto
+
+
+lemma graph_p_node_of_key_eq:
+  "rbt_sorted (rbt_of (ATBranch c k v ci li ki vi ri al ar)) \<Longrightarrow>
+  Map.graph (p_node_of_key (ATBranch c k v ci li ki vi ri al ar) p) =
+  {(k, (p, ATBranch c k v ci li ki vi ri al ar))} \<union> (Map.graph (p_node_of_key al li)) \<union> (Map.graph (p_node_of_key ar ri))"
+  apply standard
+  subgoal 
+    unfolding Map.graph_def
+    apply standard
+    apply simp
+    by (metis assn_tree.sel(2,5,8,9,10) linorder_neq_iff option.inject)
+  subgoal premises prems
+  proof
+    fix x
+    let ?br = "ATBranch c k v ci li ki vi ri al ar"
+    assume asm: "x \<in> {(k, p, ?br)} \<union> Map.graph (p_node_of_key al li) \<union> Map.graph (p_node_of_key ar ri)"
+    obtain xk xp xbr where ab: "x = (xk, xp, xbr)" using prod_cases3 .
+
+    have "xk \<guillemotleft>| rbt_of ar" and "rbt_of al |\<guillemotleft> xk" if "xk = k" using prems that by simp+
+    hence "x \<in> {(k, p, ?br)}" if "xk = k"
+      using that p_node_of_key_greater_none p_node_of_key_less_none asm in_graphD ab
+      by (metis Un_iff option.distinct(1))
+
+    hence center: "p_node_of_key ?br p k = Some (xp, xbr)" if "xk = k" using that ab by simp
+
+
+    from ab have lnot1: "x \<notin> {(k, p, ?br)}" if "xk < k" using that by blast
+
+    have "xk \<guillemotleft>| rbt_of ar" if "xk < k" using that prems rbt_greater_trans by auto
+    hence "p_node_of_key ar ri xk = None" if "xk < k" using that ptr_of_key_greater_none by auto
+    with ab have lnot3: "x \<notin> Map.graph (p_node_of_key ar ri)" if "xk < k" using that in_graphD by fastforce
+
+    from lnot1 lnot3 asm ab have left: "p_node_of_key al li xk = Some (xp, xbr)" if "xk < k" using that in_graphD by fast
+
+
+    have right: "p_node_of_key ar ri xk = Some (xp, xbr)" if "xk > k" 
+      using that in_graphD p_node_of_key_less_none prems rbt_less_trans asm ab
+      by (metis (no_types, opaque_lifting) Un_iff dual_order.irrefl empty_iff insert_iff option.distinct(1) prod.sel(1) rbt_of.simps(2) rbt_sorted.simps(2))
+
+
+    from center left right show "x \<in> Map.graph (p_node_of_key ?br p)"
+      apply (cases xk k rule: linorder_cases)
+      using ab apply (auto intro!: in_graphI)
+      done
+  qed
+  done
+
+lemma ptr_of_key_node_p_of_key_eq:
+  "Map.graph (ptr_of_key t ti) = { (a, fst b) | a b. (a, b) \<in> Map.graph (p_node_of_key t ti) } "
+  unfolding Map.graph_def
+  by simp
+
+lemma graph_ptr_of_key_eq:
+  "rbt_sorted (rbt_of (ATBranch c k v ci li ki vi ri al ar)) \<Longrightarrow>
+  Map.graph (ptr_of_key (ATBranch c k v ci li ki vi ri al ar) p) =
+  {(k,p)} \<union> (Map.graph (ptr_of_key al li)) \<union> (Map.graph (ptr_of_key ar ri))"
+  apply (simp add: ptr_of_key_node_p_of_key_eq)
+  using graph_p_node_of_key_eq by fastforce
+
+
+lemma fun_eq_graphI:
+  "Map.graph f = Map.graph g \<Longrightarrow> f = g"
+  unfolding Map.graph_def
+  apply standard
+  subgoal for x 
+    apply (cases "f x"; cases "g x")
+       apply force+
+    done
+  done
+
+
+
+lemma at_ptr_graph_graph_eq:
+  "rbt_sorted (rbt_of t) \<Longrightarrow> at_ptr_graph t p = Map.graph (ptr_of_key t p)"
+  apply (induction t arbitrary: p)
+  subgoal
+    unfolding Map.graph_def
+    apply simp
+    done
+  subgoal premises prems for x1 x2 x3 x4 x5 x6 x7 x8 t1 t2 p
+  proof -
+    from prems have "at_ptr_graph t1 p = Map.graph (ptr_of_key t1 p)" by auto
+    moreover from prems have "at_ptr_graph t2 p = Map.graph (ptr_of_key t2 p)" by auto
+
+    ultimately show ?thesis
+      using prems graph_ptr_of_key_eq
+      by fastforce
+  qed
+  done
+
+lemma ptr_of_key_eqI [intro!]:
+  "\<lbrakk>rbt_sorted (rbt_of t); rbt_sorted (rbt_of t'); at_ptr_graph t p = at_ptr_graph t' p'\<rbrakk>
+   \<Longrightarrow> ptr_of_key t p = ptr_of_key t' p'"
+  using at_ptr_graph_graph_eq fun_eq_graphI by metis
+
+lemma ptr_of_key_subsetI [intro!]:
+  "\<lbrakk>rbt_sorted (rbt_of t); rbt_sorted (rbt_of t'); at_ptr_graph t p \<subseteq> at_ptr_graph t' p'\<rbrakk>
+   \<Longrightarrow> ptr_of_key t p \<subseteq>\<^sub>m ptr_of_key t' p'"
+  apply (simp add: at_ptr_graph_graph_eq) 
+  unfolding map_le_def Map.graph_def
+  by fastforce
+
+declare ptr_of_key.simps[simp del]
+
+lemma ptr_of_key_subsetD:
+  "\<lbrakk>ptr_of_key t ti \<subseteq>\<^sub>m ptr_of_key t' ti'; rbt_sorted (rbt_of t); rbt_sorted (rbt_of t')\<rbrakk> 
+    \<Longrightarrow> at_ptr_graph t ti \<subseteq> at_ptr_graph t' ti'"
+  apply (simp add: at_ptr_graph_graph_eq)
+  unfolding map_le_def Map.graph_def by force
+
+subsection \<open>value_of_key\<close>
+
+fun value_of_key where
+  "value_of_key t ti k = map_option (assn_tree.ll_val \<circ> snd) (p_node_of_key t ti k)"
+
+declare value_of_key.simps[simp del]
+
+end
+
+end
