LLVM_DS_RBT/Delete/Alloc_Optimized/Balance_Opt_LR.thy
@@ -1,0 +1,274 @@
+theory Balance_Opt_LR
+  imports
+    "../Balance_LR"
+    "../../Insert/Alloc_Optimized/Insert_Opt"
+begin
+
+
+context rbt_impl
+begin
+interpretation rbt_impl_deps .
+
+
+definition "bl_opt_case_1 n_p \<equiv>
+  do {
+    l_p \<leftarrow> left n_p;
+    set_color_p 0 n_p;
+    set_color_p 1 l_p;
+    return n_p
+  }
+"
+
+
+definition "bl_opt_case_2 n_p \<equiv>
+  do {
+    r_p \<leftarrow> right n_p;
+    set_color_p 0 r_p;
+    set_color_p 1 n_p;
+    balance_opt n_p
+  }
+"
+
+
+definition "bl_opt_case_3 n_p \<equiv>
+  do {
+    r_p \<leftarrow> right n_p;
+
+    r_p \<leftarrow> rotate_right r_p;
+    set_right_p r_p n_p;
+
+    n2_p \<leftarrow> rotate_left n_p;
+    
+    r_p \<leftarrow> right n2_p;
+    rr_p \<leftarrow> right r_p;
+    (if rr_p = null then return () else set_color_p 0 rr_p);
+
+    set_color_p 1 r_p;
+    r_p \<leftarrow> balance_opt r_p;
+    set_right_p r_p n2_p;
+
+    set_color_p 1 n_p;
+    set_color_p 0 n2_p;
+    return n2_p
+  }
+"
+
+
+definition "balance_left_opt n_p \<equiv> 
+  do {
+    n \<leftarrow> ll_load n_p;
+    case n of (RBT_NODE _ l_p k v r_p) \<Rightarrow>
+    if! ll_matches_rbt bl_pat_1 l_p
+    then! bl_opt_case_1 n_p
+    else! if! ll_matches_rbt bl_pat_2 r_p
+    then! bl_opt_case_2 n_p
+    else! if! ll_matches_rbt bl_pat_3 r_p
+    then! bl_opt_case_3 n_p
+    else! do { 
+      free n_p;
+      empty
+    }
+  }"
+
+
+lemma balance_left_opt_correct [vcg_rules]:
+  "
+    llvm_htriple
+    (
+      rbt_assn l li **
+      \<upharpoonleft>key_assn k ki **
+      \<upharpoonleft>value_assn v vi **
+      rbt_assn r ri **
+      color_assn c ci **
+      \<upharpoonleft>ll_bpto (RBT_NODE ci li ki vi ri) n_p
+    )
+    (balance_left_opt n_p)
+    (\<lambda>res. rbt_assn (rbt_balance_left l k v r) res)
+  "
+  unfolding 
+    balance_left_opt_def
+    bl_opt_case_1_def
+    bl_opt_case_2_def
+    bl_opt_case_3_def
+    rotate_left_def
+    rotate_right_def
+    left_def
+    right_def
+
+  apply vcg
+  subgoal (*case 1*)
+    apply (cases "(l, k, v, r)" rule: RBT_Impl.balance_left.cases)
+              apply auto
+    apply vcg
+    done
+  subgoal (*case 2+*)
+    apply vcg
+
+    subgoal (*case 2*)
+      apply (cases "(l, k, v, r)" rule: RBT_Impl.balance_left.cases)
+                apply auto
+       apply vcg
+      done
+    subgoal (*case 3+*)
+      apply vcg
+      subgoal (*case 3*)
+        apply (cases "(l, k, v, r)" rule: RBT_Impl.balance_left.cases)
+                  apply auto
+         apply vcg
+         supply load_rbt_non_null[vcg_rules]
+         apply vcg
+        done
+      subgoal (*case 4*)
+        apply (cases "(l, k, v, r)" rule: RBT_Impl.balance_left.cases)
+                  apply auto
+        apply (
+            vcg |
+            vcg_solve |
+            vcg_rl, vcg_compat, (sepwith simp | simp)+
+            )+
+        done
+      done
+    done
+  done
+
+
+definition "br_opt_case_1 n_p \<equiv>
+  do {
+    l_p \<leftarrow> right n_p;
+    set_color_p 0 n_p;
+    set_color_p 1 l_p;
+    return n_p
+  }
+"
+
+
+definition "br_opt_case_2 n_p \<equiv>
+  do {
+    r_p \<leftarrow> left n_p;
+    set_color_p 0 r_p;
+    set_color_p 1 n_p;
+    balance_opt n_p
+  }
+"
+
+
+definition "br_opt_case_3 n_p \<equiv>
+  do {
+    r_p \<leftarrow> left n_p;
+
+    r_p \<leftarrow> rotate_left r_p;
+    set_left_p r_p n_p;
+
+    n2_p \<leftarrow> rotate_right n_p;
+    
+    r_p \<leftarrow> left n2_p;
+    rr_p \<leftarrow> left r_p;
+    (if rr_p = null then return () else set_color_p 0 rr_p);
+
+    set_color_p 1 r_p;
+    r_p \<leftarrow> balance_opt r_p;
+    set_left_p r_p n2_p;
+
+    set_color_p 1 n_p;
+    set_color_p 0 n2_p;
+    return n2_p
+  }
+"
+
+
+definition "balance_right_opt n_p \<equiv> 
+  do {
+    n \<leftarrow> ll_load n_p;
+    case n of (RBT_NODE _ l_p k v r_p) \<Rightarrow>
+    if! ll_matches_rbt br_pat_1 r_p
+    then! br_opt_case_1 n_p
+    else! if! ll_matches_rbt br_pat_2 l_p
+    then! br_opt_case_2 n_p
+    else! if! ll_matches_rbt br_pat_3 l_p
+    then! br_opt_case_3 n_p
+    else! do { 
+      free n_p;
+      empty
+    }
+  }"
+
+
+lemma balance_right_opt_correct [vcg_rules]:
+  "
+    llvm_htriple
+    (
+      rbt_assn l li **
+      \<upharpoonleft>key_assn k ki **
+      \<upharpoonleft>value_assn v vi **
+      rbt_assn r ri **
+      color_assn c ci **
+      \<upharpoonleft>ll_bpto (RBT_NODE ci li ki vi ri) n_p
+    )
+    (balance_right_opt n_p)
+    (\<lambda>res. rbt_assn (rbt_balance_right l k v r) res)
+  "
+  unfolding 
+    balance_right_opt_def
+    br_opt_case_1_def
+    br_opt_case_2_def
+    br_opt_case_3_def
+    rotate_right_def
+    rotate_left_def
+    right_def
+    left_def
+
+  apply vcg
+  subgoal (*case 1*)
+    apply (cases "(l, k, v, r)" rule: RBT_Impl.balance_right.cases)
+              apply auto
+    apply vcg
+    done
+  subgoal (*case 2+*)
+    apply vcg
+
+    subgoal (*case 2*)
+      apply (cases "(l, k, v, r)" rule: RBT_Impl.balance_right.cases)
+                apply auto
+       apply vcg
+      done
+    subgoal (*case 3+*)
+      apply vcg
+      subgoal (*case 3*)
+        apply (cases "(l, k, v, r)" rule: RBT_Impl.balance_right.cases)
+                  apply auto
+         apply vcg
+         supply load_rbt_non_null[vcg_rules]
+         apply vcg
+        done
+      subgoal (*case 4*)
+        apply (cases "(l, k, v, r)" rule: RBT_Impl.balance_right.cases)
+                  apply auto
+        apply (
+            vcg |
+            vcg_solve |
+            vcg_rl, vcg_compat, (sepwith simp | simp)+
+            )+
+        done
+      done
+    done
+  done
+
+
+lemmas [llvm_inline] = 
+  br_opt_case_1_def
+  br_opt_case_2_def
+  br_opt_case_3_def
+  bl_opt_case_1_def
+  bl_opt_case_2_def
+  bl_opt_case_3_def
+
+
+lemmas [llvm_code] =
+  balance_right_opt_def
+  balance_left_opt_def
+
+
+end
+
+
+end
