LLVM_DS_RBT/Delete/Alloc_Optimized/Combine_Opt.thy
@@ -1,5 +1,7 @@
-theory Combine
-  imports Balance_LR
+theory Combine_Opt
+  imports        
+  "../Combine"
+  "Balance_Opt_LR"
 begin
 
 
@@ -8,16 +10,9 @@ begin
 interpretation rbt_impl_deps .
 
 
-abbreviation "is_black_b x \<equiv> matches_rbt (RP_Branch CP_B RP_Var RP_Var) x"
-abbreviation "is_red_b x \<equiv> matches_rbt (RP_Branch CP_R RP_Var RP_Var) x"
-
-abbreviation "ll_is_black_br x \<equiv> ll_matches_rbt (RP_Branch CP_B RP_Var RP_Var) x"
-abbreviation "ll_is_red_br x \<equiv> ll_matches_rbt (RP_Branch CP_R RP_Var RP_Var) x"
-
-
-partial_function (M) combine ::
+partial_function (M) combine_opt ::
   "('ki, 'vi) rbti \<Rightarrow> ('ki, 'vi) rbti \<Rightarrow> ('ki, 'vi) rbti llM" where
-  "combine l_p r_p = do {
+  "combine_opt l_p r_p = do {
     if l_p = null then return r_p
     else if r_p = null then return l_p
     else do {
@@ -25,7 +20,7 @@ partial_function (M) combine ::
       r \<leftarrow> ll_load r_p;
       if rbt_node.color l = rbt_node.color r
       then do {
-        combined_p \<leftarrow> combine (rbt_node.right l) (rbt_node.left r);
+        combined_p \<leftarrow> combine_opt (rbt_node.right l) (rbt_node.left r);
         is_red_b \<leftarrow> ll_is_red_br combined_p;
         if is_red_b = ll_True then
         do {
@@ -46,22 +41,19 @@ partial_function (M) combine ::
             return l_p
           }
           else do {
-            case l of (RBT_NODE _ ll lk lv _) \<Rightarrow>
-            do {
-              ll_free l_p;
-              balance_left ll lk lv r_p
-            }
+            set_right_p r_p l_p;
+            balance_left_opt l_p
           }
         }
       }
       else if (rbt_node.color r = 0)
       then do {
-        combined_p \<leftarrow> combine l_p (rbt_node.left r);
+        combined_p \<leftarrow> combine_opt l_p (rbt_node.left r);
         set_left_p combined_p r_p;
         return r_p
       }
       else do { 
-        combined_p \<leftarrow> combine (rbt_node.right l) r_p;
+        combined_p \<leftarrow> combine_opt (rbt_node.right l) r_p;
         set_right_p combined_p l_p;
         return l_p
       }
@@ -69,30 +61,30 @@ partial_function (M) combine ::
   }"
 
 
-lemma combine_correct [vcg_rules]:
+lemma combine_opt_correct [vcg_rules]:
   "
   llvm_htriple
   (rbt_assn l li ** rbt_assn r ri)
-  (combine li ri)
+  (combine_opt li ri)
   (\<lambda>x. rbt_assn (rbt_combine l r) x)
 "
 proof(induction l r arbitrary: li ri rule: RBT_Impl.combine.induct)
   case (1 x)
   then show ?case 
-    apply (subst combine.simps)
+    apply (subst combine_opt.simps)
     apply vcg
     done
 next
   case (2 v va vb vc vd)
   then show ?case 
-    apply (subst combine.simps)
+    apply (subst combine_opt.simps)
     apply vcg
     done
 next
   case (3 a k x b c s y d)
   note [vcg_rules] = 3
   show ?case
-    apply (subst combine.simps)
+    apply (subst combine_opt.simps)
     apply vcg
     subgoal
       apply resolve_rbt_pat_mat
@@ -109,7 +101,7 @@ next
   case (4 a k x b c s y d)
   note [vcg_rules] = 4
   show ?case
-    apply (subst combine.simps)
+    apply (subst combine_opt.simps)
     apply vcg
     subgoal
       apply resolve_rbt_pat_mat
@@ -126,20 +118,20 @@ next
   case (5 va vb vc vd b k x c)
   note [vcg_rules] = 5
   show ?case
-    apply (subst combine.simps)
+    apply (subst combine_opt.simps)
     apply vcg
     done
 next
   case (6 a k x b va vb vc vd)
   note [vcg_rules] = 6
   show ?case
-    apply (subst combine.simps)
+    apply (subst combine_opt.simps)
     apply vcg
     done
 qed
 
 
-lemmas [llvm_code] = combine.simps
+lemmas [llvm_code] = combine_opt.simps
 
 
 end
