LLVM_DS_RBT/Delete/Alloc_Optimized/Delete_Opt.thy
@@ -1,0 +1,130 @@
+theory Delete_Opt
+  imports 
+    "Combine_Opt"
+    "../Delete"
+begin
+
+
+context rbt_impl
+begin
+interpretation rbt_impl_deps .
+
+
+partial_function (M) del_opt ::
+  "'ki \<Rightarrow> ('ki, 'vi) rbti \<Rightarrow> (('ki, 'vi) rbti) llM" where
+  "del_opt x t_p =
+  do {
+    if t_p = null then return null
+    else do {
+      t \<leftarrow> ll_load t_p;
+      case t of (RBT_NODE c a y s b) \<Rightarrow>
+      do {
+        if! lt_impl x y
+        then! do {
+          cond \<leftarrow> ll_is_black_br a;
+          l_del \<leftarrow> del_opt x a;
+          set_left_p l_del t_p;
+          if cond = 1
+          then do {balance_left_opt t_p}
+          else do {set_color_p 0 t_p; return t_p}
+        }
+        else! if! lt_impl y x
+        then! do {
+          cond \<leftarrow> ll_is_black_br b;
+          r_del \<leftarrow> del_opt x b;
+          set_right_p r_del t_p;
+          if cond = 1
+          then do {balance_right_opt t_p }
+          else do {set_color_p 0 t_p; return t_p}
+        }
+        else! do {
+            key_delete y;
+            value_delete s;
+            ll_free t_p;
+            combine a b
+        }
+      }
+    }
+  }"
+
+
+lemmas [llvm_code] = del_opt.simps
+
+
+lemma del_opt_correct':
+"
+  llvm_htriple
+  (\<upharpoonleft>key_assn k ki ** rbt_assn t ti)
+  (del_opt ki ti)
+  (\<lambda>r. rbt_assn (rbt_del_ad k t) r ** \<upharpoonleft>key_assn k ki)
+"
+proof(induct k t arbitrary: ki ti rule: rbt_del_ad.induct)
+  case (1 x)
+  then show ?case
+    apply (subst del_opt.simps)
+    apply vcg
+    done
+next
+  case (2 x c a y s b)
+
+  have IH1: 
+    "x < y \<Longrightarrow> llvm_htriple
+      (\<upharpoonleft>key_assn x ki \<and>* rbt_assn a ti)
+      (del_opt ki ti)
+      (\<lambda>r. rbt_assn (rbt_del_ad x a) r \<and>* \<upharpoonleft>key_assn x ki)"
+    for ki ti
+    using 2(1-2) by fast
+
+  have IH2:
+    "y < x \<Longrightarrow> llvm_htriple
+      (\<upharpoonleft>key_assn x ki \<and>* rbt_assn b ti)
+      (del_opt ki ti)
+      (\<lambda>r. rbt_assn (rbt_del_ad x b) r \<and>* \<upharpoonleft>key_assn x ki)"
+    for ki ti using 2(3-4) by fastforce
+
+  note [vcg_rules] = IH1 IH2
+
+  show ?case
+    apply (subst del_opt.simps)
+    apply vcg
+    done
+qed
+
+
+lemma del_opt_correct:
+"
+  llvm_htriple
+  (\<upharpoonleft>key_assn k ki ** rbt_assn t ti)
+  (del_opt ki ti)
+  (\<lambda>r. rbt_assn (rbt_del k t) r ** \<upharpoonleft>key_assn k ki)
+"
+  using del_opt_correct' rbt_del_ad_correct by metis
+
+
+definition "delete_opt x t \<equiv> do { 
+  del_res \<leftarrow> del_opt x t;
+  (if del_res = null then return () else set_color_p 1 del_res);
+  return del_res 
+  }"
+
+
+lemmas [llvm_code] = delete_opt_def
+
+
+lemma delete_opt_correct [vcg_rules]:
+"
+  llvm_htriple
+  (\<upharpoonleft>key_assn k ki ** rbt_assn t ti)
+  (delete_opt ki ti)
+  (\<lambda>r. rbt_assn (rbt_delete k t) r ** \<upharpoonleft>key_assn k ki)
+"
+  unfolding delete_opt_def rbt_delete_def paint_def
+  supply del_opt_correct[vcg_rules] load_rbt_non_null[vcg_rules]
+  apply vcg
+  done
+
+
+end
+
+
+end
