LLVM_DS_RBT/Export_Wrappers.thy
@@ -1,12 +1,13 @@
 theory Export_Wrappers
-  imports Map_Interface
+  imports 
+    Map_Interface
+    "Insert/Alloc_Optimized/Insert_Opt"
+    "Delete/Alloc_Optimized/Delete_Opt"
 begin
 
 
 context rbt_map
 begin
-
-
 interpretation monad_syntax_M_loc .
 
 
@@ -51,12 +52,35 @@ definition insert_wrap :: "_ ptr \<Rightarrow> _ ptr \<Rightarrow> _ ptr \<Right
   "
 
 
+definition insert_opt_wrap :: "_ ptr \<Rightarrow> _ ptr \<Rightarrow> _ ptr \<Rightarrow> unit llM" where [llvm_code]:
+  "insert_opt_wrap rbt_p key_p value_p =
+    do {
+      rbt \<leftarrow> ll_load rbt_p;
+      key \<leftarrow> ll_load key_p;
+      value \<leftarrow> ll_load value_p;
+      res \<leftarrow> insert_opt key value rbt;
+      ll_store res rbt_p
+    }
+  "
+
+
 definition delete_wrap :: "_ ptr \<Rightarrow> _ ptr \<Rightarrow> unit llM" where [llvm_code]:
   "delete_wrap rbt_p key_p  =
     do {
       rbt \<leftarrow> ll_load rbt_p;
       key \<leftarrow> ll_load key_p;
       res \<leftarrow> delete key rbt;
+      ll_store res rbt_p
+    }
+  "
+
+
+definition delete_opt_wrap :: "_ ptr \<Rightarrow> _ ptr \<Rightarrow> unit llM" where [llvm_code]:
+  "delete_opt_wrap rbt_p key_p  =
+    do {
+      rbt \<leftarrow> ll_load rbt_p;
+      key \<leftarrow> ll_load key_p;
+      res \<leftarrow> delete_opt key rbt;
       ll_store res rbt_p
     }
   "
