LLVM_DS_RBT/Extended_Assertion.thy
@@ -1,0 +1,295 @@
+theory Extended_Assertion
+  imports Setup
+begin
+
+subsection \<open>Assertion Tree\<close>
+
+datatype ('k, 'v, 'ki, 'vi) assn_tree =
+  ATEmpty |
+  ATBranch
+  (color: color)
+  (key: 'k)
+  (val: 'v) 
+  "8 word"
+  (ll_left: "('ki, 'vi) rbti")
+  (ll_key: 'ki) 
+  (ll_val: 'vi) 
+  (ll_right: "('ki, 'vi) rbti")
+  (left: "('k, 'v, 'ki, 'vi) assn_tree")
+  (right: "('k, 'v, 'ki, 'vi) assn_tree")
+
+
+subsubsection \<open>rbt_of\<close>
+
+fun rbt_of :: "('k, 'v, 'ki, 'vi) assn_tree \<Rightarrow> ('k, 'v) rbt"  where
+  "rbt_of ATEmpty = rbt.Empty" |
+  "rbt_of (ATBranch c k v _ _ _ _ _ l r) =
+    (rbt.Branch c (rbt_of l) k v (rbt_of r))"
+
+declare rbt_of.elims[where y=rbt.Empty, simplified, elim!]
+lemma rbt_of_branchE [elim!]:
+  assumes
+    "rbt_of t = rbt.Branch c l k v r"
+  shows
+    "\<lbrakk>\<And>al ar. rbt_of al = l \<Longrightarrow> rbt_of ar = r  \<Longrightarrow> (\<And>ci li ki vi ri. t = ATBranch c k v ci li ki vi ri al ar \<Longrightarrow> P)\<rbrakk> \<Longrightarrow> P"
+  using assms
+  by (blast elim: rbt_of.elims)
+
+
+lemma rbt_of_branchI [intro!]:
+  assumes 
+    "rbt_of l = l'"
+    "rbt_of r = r'"
+  shows
+    "rbt_of (ATBranch c k v ci li ki vi ri l r) = (rbt.Branch c l' k v r')"
+  using assms by simp
+
+
+lemma rbt_of_emptyI [intro!]:
+  "rbt_of ATEmpty = rbt.Empty"
+  by simp
+
+lemma rbt_of_reorient [simp]: 
+  "(Branch c l k v r = rbt_of x) = (rbt_of x = Branch c l k v r)" by auto
+
+subsection \<open>Assertion\<close>
+
+datatype except =     
+  COLOR_EX | KEY_EX | VALUE_EX | PTO_EX
+
+fun assn_unless (infixl "unless" 40) where 
+  "assn_unless assn b = (if b then \<box> else assn)"
+declare assn_unless.simps[simp del]
+
+
+lemma assn_unless_True [simp]:
+  "(assn unless False) = assn"
+  by (simp add: assn_unless.simps)
+
+
+lemma assn_unless_False [simp]:
+  "(assn unless True) = \<box>"
+  by (simp add: assn_unless.simps)
+
+
+context rbt_impl
+begin
+interpretation rbt_impl_deps .
+
+fun rbt_assn_ext :: "('k, 'v, 'ki, 'vi) assn_tree \<Rightarrow> ('k \<times> except) set \<Rightarrow> ('ki, 'vi) rbti \<Rightarrow> ll_assn" where
+  "rbt_assn_ext ATEmpty ex p = \<up>(p = null)"
+| "rbt_assn_ext (ATBranch c k v ci li ki vi ri l r) ex p =
+    (
+      \<upharpoonleft>ll_bpto (RBT_NODE ci li ki vi ri) p unless (k, PTO_EX) \<in> ex **
+      color_assn c ci unless (k, COLOR_EX) \<in> ex **
+      rbt_assn_ext l ex li **
+      \<upharpoonleft>key_assn k ki unless (k, KEY_EX) \<in> ex **
+      \<upharpoonleft>value_assn v vi unless (k, VALUE_EX) \<in> ex **
+      rbt_assn_ext r ex ri
+    )"
+declare rbt_assn_ext.simps(2)[simp del]
+lemmas rbt_assn_ext_unfold = rbt_assn_ext.simps(2)
+
+
+lemma rbt_assn_ext_null [simp]: 
+  "(\<And>k. (k, PTO_EX) \<notin> ex) \<Longrightarrow> rbt_assn_ext t ex null = \<up>(t =  ATEmpty)"
+  apply (cases t)
+  using rbt_assn_ext_unfold apply auto
+  done
+
+lemma rbt_assn_ext_empty_set_null [simp]:
+  "rbt_assn_ext t {} null = \<up>(t  = ATEmpty)" by simp
+
+
+subsection \<open>Load Rules\<close>
+
+
+lemma load_rbt [vcg_rules]:
+  "
+    (k, PTO_EX) \<notin> ex \<Longrightarrow>
+    llvm_htriple
+    (rbt_assn_ext (ATBranch c k v ci li ki vi ri l r) ex ti)
+    (ll_load ti)
+    (\<lambda>res.
+      rbt_assn_ext (ATBranch c k v ci li ki vi ri l r) ex ti **
+      \<up>(res = RBT_NODE ci li ki vi ri)
+    )
+  "
+  unfolding rbt_assn_ext_unfold
+  apply vcg
+  done
+
+
+lemma load_rbt_non_null:
+  "
+    ti \<noteq> null \<Longrightarrow>
+    llvm_htriple
+    (rbt_assn_ext t {} ti)
+    (ll_load ti)
+    (\<lambda>res.
+      EXS ci li ki vi ri c l k v r.
+      rbt_assn_ext t {} ti **
+      \<up>(t = (ATBranch c k v ci li ki vi ri l r)) **
+      \<up>(res = RBT_NODE ci li ki vi ri)
+    )
+  "
+  apply vcg
+  apply (cases t)
+  subgoal by simp (*contradiction*)
+  subgoal by vcg
+  done
+
+subsection \<open>Reduction Rules\<close>
+
+lemma unfold_rbt_assn_ext_red_rule_1 [fri_red_rules]:
+  "
+    is_sep_red
+    (\<upharpoonleft>ll_bpto (RBT_NODE ci li ki vi ri) ti)
+    (
+        \<upharpoonleft>ll_bpto (RBT_NODE ci li ki vi ri) ti unless (k, PTO_EX) \<in> ex **
+        color_assn c ci unless (k, COLOR_EX) \<in> ex **
+        rbt_assn_ext l ex li **
+        \<upharpoonleft>key_assn k ki unless (k, KEY_EX) \<in> ex **
+        \<upharpoonleft>value_assn v vi unless (k, VALUE_EX) \<in> ex **
+        rbt_assn_ext r ex ri
+    )
+    (\<upharpoonleft>ll_bpto (RBT_NODE ci li ki vi ri) ti)
+    (rbt_assn_ext (ATBranch c k v ci li ki vi ri l r) ex ti)
+  "
+  apply (rule is_sep_redI)
+  unfolding rbt_assn_ext_unfold
+  apply simp
+  done
+
+lemma unfold_rbt_assn_ext_red_rule_2 [fri_red_rules]:
+  "
+    is_sep_red
+    (\<upharpoonleft>ll_bpto (RBT_NODE ci li ki vi ri) ti unless cond)
+    (
+        \<upharpoonleft>ll_bpto (RBT_NODE ci li ki vi ri) ti unless (k, PTO_EX) \<in> ex **
+        color_assn c ci unless (k, COLOR_EX) \<in> ex **
+        rbt_assn_ext l ex li **
+        \<upharpoonleft>key_assn k ki unless (k, KEY_EX) \<in> ex **
+        \<upharpoonleft>value_assn v vi unless (k, VALUE_EX) \<in> ex **
+        rbt_assn_ext r ex ri
+    )
+    (\<upharpoonleft>ll_bpto (RBT_NODE ci li ki vi ri) ti unless cond)
+    (rbt_assn_ext (ATBranch c k v ci li ki vi ri l r) ex ti)
+  "
+  apply (rule is_sep_redI)
+  unfolding rbt_assn_ext_unfold
+  apply simp
+  done
+
+
+lemma rbt_assn_ext_key_assn_unfold [fri_red_rules]: 
+  "
+    is_sep_red
+    (
+      \<upharpoonleft>ll_bpto (RBT_NODE ci li ki vi ri) ti \<and>*
+      color_assn c ci \<and>* rbt_assn_ext l {} li \<and>*
+      \<upharpoonleft>value_assn v vi \<and>*
+      rbt_assn_ext r {} ri)
+    \<box>
+    (rbt_assn_ext (ATBranch c k v ci li ki vi ri l r) {} ti)
+    (\<upharpoonleft>key_assn k ki)
+  "
+  apply (rule is_sep_redI)
+  unfolding rbt_assn_ext_unfold
+  apply simp
+  subgoal premises prems
+    apply (sep isep_dest: prems)
+    done
+  done
+
+
+lemma rbt_assn_ext_color_assn_unfold [fri_red_rules]: 
+  "
+    is_sep_red
+    (
+      \<upharpoonleft>ll_bpto (RBT_NODE ci li ki vi ri) ti \<and>*
+      rbt_assn_ext l {} li \<and>*
+      \<upharpoonleft>key_assn k ki **
+      \<upharpoonleft>value_assn v vi \<and>*
+      rbt_assn_ext r {} ri)
+    \<box>
+    (rbt_assn_ext (ATBranch c k v ci li ki vi ri l r) {} ti)
+    (color_assn c ci)
+  "
+  apply (rule is_sep_redI)
+  unfolding rbt_assn_ext_unfold
+  apply simp
+  subgoal premises prems
+    apply (sep isep_dest: prems)
+    done
+  done
+
+
+lemma rbt_assn_ext_pto_assn_unfold [fri_red_rules]:
+  "
+    is_sep_red
+    (
+      color_assn c ci **
+      rbt_assn_ext l {} li \<and>*
+      \<upharpoonleft>key_assn k ki **
+      \<upharpoonleft>value_assn v vi \<and>*
+      rbt_assn_ext r {} ri)
+    \<box>
+    (rbt_assn_ext (ATBranch c k v ci li ki vi ri l r) {} ti)
+    (\<upharpoonleft>ll_bpto (RBT_NODE ci li ki vi ri) ti)
+  "
+  apply (rule is_sep_redI)
+  unfolding rbt_assn_ext_unfold
+  apply simp
+  subgoal premises prems
+    apply (sep isep_dest: prems)
+    done
+  done
+
+
+lemma rbt_assn_ext_left_assn_unfold [fri_red_rules]:
+  "
+    is_sep_red
+    (
+      \<upharpoonleft>ll_bpto (RBT_NODE ci li ki vi ri) ti unless (k, PTO_EX) \<in> ex **
+      color_assn c ci unless (k, COLOR_EX) \<in> ex **
+      \<upharpoonleft>key_assn k ki unless (k, KEY_EX) \<in> ex **
+      \<upharpoonleft>value_assn v vi unless (k, VALUE_EX) \<in> ex \<and>*
+      rbt_assn_ext r ex ri)
+    \<box>
+    (rbt_assn_ext (ATBranch c k v ci li ki vi ri l r) ex ti)
+    (rbt_assn_ext l ex li)
+  "
+  apply (rule is_sep_redI)
+  unfolding rbt_assn_ext_unfold
+  apply simp
+  subgoal premises prems
+    apply (sep isep_dest: prems)
+    done
+  done
+
+lemma rbt_assn_ext_right_assn_unfold [fri_red_rules]:
+  "
+    is_sep_red
+    (
+      \<upharpoonleft>ll_bpto (RBT_NODE ci li ki vi ri) ti unless (k, PTO_EX) \<in> ex **
+      color_assn c ci unless (k, COLOR_EX) \<in> ex **
+      rbt_assn_ext l ex li **
+      \<upharpoonleft>key_assn k ki unless (k, KEY_EX) \<in> ex **
+      \<upharpoonleft>value_assn v vi unless (k, VALUE_EX) \<in> ex
+    )
+    \<box>
+    (rbt_assn_ext (ATBranch c k v ci li ki vi ri l r) ex ti)
+    (rbt_assn_ext r ex ri)
+  "
+  apply (rule is_sep_redI)
+  unfolding rbt_assn_ext_unfold
+  apply simp
+  subgoal premises prems
+    apply (sep isep_dest: prems)
+    done
+  done
+
+end
+
+end
