LLVM_DS_RBT/Extended_Assertion_Exceptions.thy
@@ -1,0 +1,136 @@
+theory Extended_Assertion_Exceptions
+  imports 
+    Abstract_Rbt
+    Assertion_Tree_Lookup
+begin
+
+context rbt_impl
+begin
+
+lemma rbt_less_value_ex_eq_2 [simp]:
+  "rbt_of t |\<guillemotleft> kn \<Longrightarrow> rbt_assn_ext t (ex - {(kn, VALUE_EX)}) ti = rbt_assn_ext t ex ti"
+proof (induction t arbitrary: ti)
+  case ATEmpty
+  show ?case by simp
+next
+  case (ATBranch c k v ci li ki vi ri l r)
+
+  hence "kn \<noteq> k" by auto  
+  
+  with ATBranch show ?case
+    unfolding rbt_assn_ext_unfold
+    apply simp
+    done
+qed
+
+lemma rbt_less_value_ex_eq_1 [simp]:
+  "rbt_of t |\<guillemotleft> kn \<Longrightarrow> rbt_assn_ext t (Set.insert (kn, VALUE_EX) ex) ti = rbt_assn_ext t ex ti"
+  apply (subst rbt_less_value_ex_eq_2[symmetric]) by simp+
+
+lemma rbt_greater_value_ex_eq_2 [simp]:
+  "kn \<guillemotleft>| rbt_of t \<Longrightarrow> rbt_assn_ext t (ex - {(kn, VALUE_EX)}) ti = rbt_assn_ext t ex ti"
+proof (induction t arbitrary: ti)
+  case ATEmpty
+  show ?case by simp
+next
+  case (ATBranch c k v ci li ki vi ri l r)
+
+  hence "kn \<noteq> k" by auto  
+  
+  with ATBranch show ?case
+    unfolding rbt_assn_ext_unfold
+    apply simp
+    done
+qed
+
+lemma rbt_greater_value_ex_eq_1 [simp]:
+  "kn \<guillemotleft>| rbt_of t \<Longrightarrow> rbt_assn_ext t (Set.insert (kn, VALUE_EX) ex) ti = rbt_assn_ext t ex ti"
+  apply (subst rbt_greater_value_ex_eq_2[symmetric]) by simp+
+
+lemma value_ex_join_ent:
+  assumes
+    "(kn, VALUE_EX) \<in> ex" and
+    "value_of_key t1 ti kn = Some vi" and
+    "rbt_sorted (rbt_of t1)"
+  shows
+    "
+    rbt_assn_ext t1 ex ti ** \<upharpoonleft>value_assn v vi \<turnstile> 
+    (EXS t2. rbt_assn_ext t2 (ex - {(kn, VALUE_EX)}) ti ** \<up>(rbt_of t2 = rbt_update (rbt_of t1) kn v))
+    "
+  using assms
+proof (induction t1 arbitrary: ti)
+  case ATEmpty
+  then show ?case unfolding value_of_key.simps by simp
+next
+  case (ATBranch c k v ci li ki vi ri l r)
+  show ?case
+  proof(cases kn k rule: linorder_cases)
+    case less
+    note ATBranch(2)[isep_dest]
+
+    from less have "kn \<noteq> k" by simp
+    moreover from ATBranch(5) rbt_greater_trans less have "kn \<guillemotleft>| rbt_of r" by auto
+
+    ultimately show ?thesis using ATBranch(3-4) less
+      apply - 
+      unfolding rbt_assn_ext_unfold
+      apply (isep_drule drule: ATBranch(1))
+      using ATBranch(5) apply (auto simp add: value_of_key.simps)[3]
+      apply sepE
+       apply auto[]
+      apply auto[]
+      apply sep
+      done
+  next
+    case equal
+    with ATBranch(4) show ?thesis
+      apply -
+      apply sepE
+       apply auto[]
+      unfolding rbt_assn_ext_unfold
+      apply sep
+      using ATBranch(5) rbt_less_trans rbt_greater_trans apply auto[]
+      using ATBranch(3) apply (simp add: value_of_key.simps) 
+      apply sep
+      done
+  next
+    case greater
+    note ATBranch(2)[isep_dest]
+
+    from greater have "\<not>kn < k" by simp
+    moreover from greater have "kn \<noteq> k" by simp
+    moreover from ATBranch(5) rbt_less_trans greater have "rbt_of l |\<guillemotleft> kn" by auto
+
+    ultimately show ?thesis using ATBranch(3-4) greater
+      apply - 
+      unfolding rbt_assn_ext_unfold
+      apply (isep_drule drule: ATBranch(2)) 
+      using ATBranch(5) apply (auto simp add: order_less_not_sym value_of_key.simps)[3]
+      apply sepE
+       apply auto[]
+      apply auto[]
+      apply sep
+      done
+  qed
+qed
+
+lemma value_ex_join_red:
+  "rbt_sorted (rbt_of t1) \<Longrightarrow> (k, VALUE_EX) \<in> ex \<Longrightarrow> (k, VALUE_EX) \<notin> ex' \<Longrightarrow> value_of_key t1 ti k = Some vi \<Longrightarrow>
+  is_sep_red
+  (EXS t2. rbt_assn_ext t2 (ex - {(k, VALUE_EX)}) ti ** \<up>(rbt_of t2 = rbt_update (rbt_of t1) k v))
+  (EXS t3. rbt_assn_ext t3 ex' ti)
+  (rbt_assn_ext t1 ex ti ** \<upharpoonleft>value_assn v vi)
+  (EXS t3. rbt_assn_ext t3 ex' ti)
+  "
+  apply (rule is_sep_redI)
+  subgoal premises prems for Ps Qs
+  apply (rule entails_trans[OF _ prems(5)])
+    apply (isep_drule drule: value_ex_join_ent)
+    using prems(1-4) apply auto[3]
+    apply (sepEwith ignore)
+    done
+  done
+
+end
+
+end
