LLVM_DS_RBT/Insert/Alloc_Optimized/Insert_Opt.thy
@@ -1,0 +1,288 @@
+theory Insert_Opt
+  imports "../Insert"
+begin
+
+
+context rbt_impl
+begin
+interpretation rbt_impl_deps .
+
+
+definition "balance_opt_case_1 n_p \<equiv> 
+  do {
+    n \<leftarrow> ll_load n_p;
+    set_color_p 0 n_p;
+    set_color_p 1 (rbt_node.left n);
+    set_color_p 1 (rbt_node.right n);
+    return n_p
+  }"
+
+
+definition "rotate_left n_p \<equiv>
+  do {
+    r_p \<leftarrow> right n_p;
+    rl_p \<leftarrow> left r_p;
+    set_left_p n_p r_p;
+    set_right_p rl_p n_p;
+    return r_p
+  }
+"
+
+
+definition "rotate_right n_p \<equiv>
+  do {
+    l_p \<leftarrow> left n_p;
+    lr_p \<leftarrow> right l_p;
+    set_right_p n_p l_p;
+    set_left_p lr_p n_p;
+    return l_p
+  }
+"
+                            
+definition "balance_opt_case_2 n_p \<equiv> 
+  do {
+    n2_p \<leftarrow> rotate_right n_p;
+    l_p \<leftarrow> left n2_p;
+    set_color_p 1 l_p;
+    return n2_p
+  }"
+
+
+definition "balance_opt_case_3 n_p \<equiv> 
+  do {
+    l_p \<leftarrow> left n_p;
+    l2_p \<leftarrow> rotate_left l_p;
+    set_left_p l2_p n_p;
+    n2_p \<leftarrow> rotate_right n_p;
+    set_color_p 1 l_p;
+    return n2_p
+  }"
+
+
+definition "balance_opt_case_4 n_p \<equiv> 
+  do {
+    n2_p \<leftarrow> rotate_left n_p;
+    r_p \<leftarrow> right n2_p;
+    set_color_p 1 r_p;
+    return n2_p
+  }"
+
+
+definition "balance_opt_case_5 n_p \<equiv> 
+  do {
+    r_p \<leftarrow> right n_p;
+    r2_p \<leftarrow> rotate_right r_p;
+    set_right_p r2_p n_p;
+    n2_p \<leftarrow> rotate_left n_p;
+    set_color_p 1 r_p;
+    return n2_p
+  }"
+
+find_theorems ll_matches_rbt htriple
+definition "balance_opt n_p \<equiv>
+  do {
+    if! ll_matches_rbt
+        (RP_Branch CP_Var 
+          (RP_Branch CP_R RP_Var RP_Var)
+          (RP_Branch CP_R RP_Var RP_Var)
+        ) n_p
+    then! balance_opt_case_1 n_p
+    else!
+    do {
+      n \<leftarrow> ll_load n_p;
+      l_p \<leftarrow> return rbt_node.left n;
+      r_p \<leftarrow> return rbt_node.right n;
+      if! ll_matches_rbt
+        (RP_Branch CP_R (RP_Branch CP_R RP_Var RP_Var) RP_Var) l_p
+      then! balance_opt_case_2 n_p
+      else! if! ll_matches_rbt 
+        (RP_Branch CP_R RP_Var (RP_Branch CP_R RP_Var RP_Var)) l_p
+      then! balance_opt_case_3 n_p
+      else! if! ll_matches_rbt 
+        (RP_Branch CP_R RP_Var (RP_Branch CP_R RP_Var RP_Var)) r_p
+      then! balance_opt_case_4 n_p
+      else! if! ll_matches_rbt 
+        (RP_Branch CP_R (RP_Branch CP_R RP_Var RP_Var) RP_Var) r_p
+      then! balance_opt_case_5 n_p
+      else! return n_p
+    }
+  }
+"
+
+lemmas [llvm_inline] =
+    balance_opt_case_1_def
+    balance_opt_case_2_def
+    balance_opt_case_3_def
+    balance_opt_case_4_def
+    balance_opt_case_5_def
+    rotate_left_def    
+    rotate_right_def
+
+lemmas [llvm_code] = balance_opt_def
+
+
+lemma balance_opt_correct [vcg_rules]:
+  "llvm_htriple
+  (
+    \<upharpoonleft>ll_bpto (RBT_NODE ci li ki vi ri) n_p **
+    rbt_assn l li **
+    rbt_assn r ri **   
+    \<upharpoonleft>key_assn k ki **
+    \<upharpoonleft>value_assn v vi **
+    color_assn color.B ci
+  )
+  (balance_opt n_p)
+  (\<lambda>res. rbt_assn (rbt_balance l k v r) res) 
+  "
+  unfolding 
+    balance_opt_def
+    balance_opt_case_1_def
+    balance_opt_case_2_def
+    balance_opt_case_3_def
+    balance_opt_case_4_def
+    balance_opt_case_5_def
+    rotate_left_def    
+    rotate_right_def
+
+  apply vcg
+  subgoal (*Case 1*)
+    apply (cases "(l, k, v, r)" rule: RBT_Impl.balance.cases)
+                        apply auto
+    apply vcg
+    done
+  subgoal (*Case 2+*)
+    apply vcg
+    subgoal (*Case 3*)
+      apply (cases "(l, k, v, r)" rule: RBT_Impl.balance.cases)
+                          apply auto
+       apply vcg
+      done
+    subgoal (*Case 4+*)
+      apply vcg
+      subgoal (*Case 4*)
+        apply (cases "(l, k, v, r)" rule: RBT_Impl.balance.cases)
+                            apply auto
+           apply vcg
+        done
+      subgoal (*Case 5+*)
+        apply vcg
+        subgoal (*Case 5*)
+          apply (cases "(l, k, v, r)" rule: RBT_Impl.balance.cases)
+                              apply auto
+           apply vcg
+          done
+        subgoal (*Case 6*)
+          apply (cases "(l, k, v, r)" rule: RBT_Impl.balance.cases)
+                              apply auto
+                              apply vcg
+          done
+        done
+      done
+    done
+  done
+
+
+definition "balance_black n_p c \<equiv> do { if c = 1 then balance_opt n_p else return n_p }"
+
+lemmas [llvm_inline] = balance_black_def
+
+
+partial_function (M) insert'_opt ::
+  "'ki \<Rightarrow> 'vi \<Rightarrow> ('ki, 'vi) rbti \<Rightarrow> ('ki, 'vi) rbti llM" where
+  "insert'_opt k\<^sub>n v\<^sub>n n_p =
+  do {
+    if n_p = null
+    then new (RBT_NODE 0 null k\<^sub>n v\<^sub>n null)
+    else
+    do {
+      n \<leftarrow> ll_load n_p;
+      case n of (RBT_NODE c l_p k v r_p) \<Rightarrow>      
+      do {
+          if! lt_impl k\<^sub>n k
+          then! do {l_p\<^sub>n \<leftarrow> insert'_opt k\<^sub>n v\<^sub>n l_p; set_left_p l_p\<^sub>n n_p; balance_black n_p c}
+          else! if! lt_impl k k\<^sub>n
+          then! do {r_p\<^sub>n \<leftarrow> insert'_opt k\<^sub>n v\<^sub>n r_p; set_right_p r_p\<^sub>n n_p; balance_black n_p c}
+          else! do {key_delete k; value_delete v;
+                    set_key_p k\<^sub>n n_p; set_value_p v\<^sub>n n_p;
+                    return n_p}
+      }     
+    }
+  }"
+
+lemmas [llvm_code] = insert'_opt.simps
+
+lemma insert'_opt_correct:
+  "
+    llvm_htriple
+    (rbt_assn tree treei ** \<upharpoonleft>key_assn k ki ** \<upharpoonleft>value_assn v vi)
+    (insert'_opt ki vi treei)
+    (\<lambda>r. rbt_assn ((rbt_ins (\<lambda>_ _ v. v)) k v tree) r)
+  "
+proof (induction k v tree arbitrary: treei ki v rule: rbt_insert_ad'.induct)
+  case (1 k\<^sub>n v\<^sub>n)
+  then show ?case
+    apply (subst insert'_opt.simps)
+    apply vcg
+    done
+next
+  case (2 k\<^sub>n v\<^sub>n l k v r)
+  
+  note [vcg_rules] = 2
+
+  show ?case
+    apply (subst insert'_opt.simps)
+    unfolding balance_black_def
+    apply vcg
+    done
+next
+  case (3 k\<^sub>n v\<^sub>n l k v r)
+
+  note [vcg_rules] = 3
+
+  show ?case
+    apply (subst insert'_opt.simps)
+    unfolding balance_black_def
+    apply vcg
+    done
+qed
+
+
+
+lemma rbt_ins_non_empty:
+  "rbt_ins f k v t \<noteq> rbt.Empty"
+  apply (induction f k v t rule: rbt_ins.induct)
+  subgoal by simp
+  subgoal using rbt_balance_non_empty by (simp, fast)
+  subgoal by simp
+  done
+
+definition insert_opt where
+  "insert_opt k v n_p \<equiv>
+  do {
+    r_p \<leftarrow> insert'_opt k v n_p;
+    set_color_p 1 r_p;
+    return r_p
+  }"
+
+lemmas [llvm_code] = insert_opt_def
+
+lemma insert_opt_correct [vcg_rules]:
+  "
+    llvm_htriple
+    (rbt_assn tree treei ** \<upharpoonleft>key_assn k ki ** \<upharpoonleft>value_assn v vi)
+    (insert_opt ki vi treei)
+    (\<lambda>r. rbt_assn (rbt_insert k v tree) r)
+  " 
+  unfolding insert_opt_def rbt_insert_def rbt_insert_with_key_def paint_def
+  supply insert'_opt_correct[vcg_rules]
+  apply vcg
+  apply (cases "rbt_ins (\<lambda>_ _ v. v) k v tree")
+  using rbt_ins_non_empty apply fast
+  apply vcg
+  done
+
+
+end
+
+
+end
