LLVM_DS_RBT/Insert/Alloc_Optimized/Insert_Opt_Ext.thy
@@ -1,0 +1,150 @@
+theory Insert_Opt_Ext
+  imports
+    Insert_Opt  
+    "../../Utilities_Extended_Assertion"
+    "../../Assertion_Tree_Lookup"
+begin
+
+context rbt_impl
+begin
+
+lemma balance_opt_correct_ext [vcg_rules]:
+  "llvm_htriple
+  (
+    rbt_assn_ext (ATBranch color.B k v ci li ki vi ri l r) {} ti ** \<up>(rbt_sorted (rbt_of (ATBranch color.B k v ci li ki vi ri l r)))
+  )
+  (balance_opt ti)
+  (\<lambda>res. EXS res_t. rbt_assn_ext res_t {} res **
+    \<up>(rbt_of res_t = rbt_balance (rbt_of l) k v (rbt_of r)) **
+    \<up>(rbt_sorted (rbt_of res_t)) **
+    \<up>(ptr_of_key res_t res = ptr_of_key (ATBranch color.B k v ci li ki vi ri l r) ti)  
+  )
+  "
+  unfolding 
+    balance_opt_def
+    balance_opt_case_1_def
+    balance_opt_case_2_def
+    balance_opt_case_3_def
+    balance_opt_case_4_def
+    balance_opt_case_5_def
+    rotate_left_def    
+    rotate_right_def
+    right_def
+    left_def
+  supply rbt_greater_trans[intro] rbt_less_trans[intro]
+  apply vcg
+  subgoal (*Case 1*)
+    apply (cases "(rbt_of l, k, v, rbt_of r)" rule: RBT_Impl.balance.cases)
+                        apply auto
+    apply vcg
+    done
+  subgoal (*Case 2+*)
+    apply vcg
+    subgoal (*Case 2*)
+      apply (cases "(rbt_of l, k, v, rbt_of r)" rule: RBT_Impl.balance.cases)
+                          apply auto
+       apply vcg
+      done
+    subgoal (*Case 3+*)
+      apply vcg
+      subgoal (*Case 3*)
+        apply (cases "(rbt_of l, k, v, rbt_of r)" rule: RBT_Impl.balance.cases)
+                            apply auto 
+           apply vcg
+        done
+      subgoal (*Case 4+*)
+        apply vcg
+        subgoal (*Case 4*)
+          apply (cases "(rbt_of l, k, v, rbt_of r)" rule: RBT_Impl.balance.cases)
+                              apply auto
+           apply vcg
+          done
+        subgoal (*Case 5*)
+          apply (cases "(rbt_of l, k, v, rbt_of r)" rule: RBT_Impl.balance.cases)
+                              apply auto
+                              apply vcg
+          done
+        done
+      done
+    done
+  done
+
+lemma insert'_opt_correct_ext:
+  "
+    llvm_htriple
+    (rbt_assn_ext t {} ti ** \<upharpoonleft>key_assn k ki ** \<upharpoonleft>value_assn v vi ** \<up>(rbt_sorted (rbt_of t)))
+    (insert'_opt ki vi ti)
+    (\<lambda>res. EXS res_t. rbt_assn_ext res_t {} res **
+      \<up>(rbt_of res_t = (rbt_ins (\<lambda>_ _ v. v)) k v (rbt_of t)) **
+      \<up>(rbt_sorted (rbt_of res_t)) **
+      \<up>(ptr_of_key t ti \<subseteq>\<^sub>m ptr_of_key res_t res)
+    )
+  "
+  supply ptr_of_key_subsetD[dest!]
+proof (induction k v "rbt_of t" arbitrary: ti t rule: rbt_insert_ad'.induct )
+  case (1 k\<^sub>n v\<^sub>n)
+  then show ?case
+    apply (subst insert'_opt.simps)
+    supply load_rbt_non_null[vcg_rules]
+    apply vcg
+    done
+next
+  case (2 k\<^sub>n v\<^sub>n l k v r)
+
+  note [vcg_rules] = 2(1-2)
+
+  from 2(3) show ?case
+    apply (subst insert'_opt.simps)
+    unfolding balance_black_def
+    supply load_rbt_non_null[vcg_rules]
+    apply (vcg;fail)
+    done
+next
+  case (3 k\<^sub>n v\<^sub>n l k v r)
+
+  note [vcg_rules] = 3(1-2)
+
+  from 3(3) show ?case
+    apply (subst insert'_opt.simps)
+    unfolding balance_black_def
+    supply load_rbt_non_null[vcg_rules] 
+    apply (vcg;fail)
+    done
+qed
+
+
+lemma insert_opt_correct_ext [vcg_rules]:
+  "
+    llvm_htriple
+    (rbt_assn_ext t {} ti ** \<upharpoonleft>key_assn k ki ** \<upharpoonleft>value_assn v vi ** \<up>(rbt_sorted (rbt_of t)))
+    (insert_opt ki vi ti)
+    (\<lambda>res_ti. EXS res_t.
+      rbt_assn_ext res_t {} res_ti **
+      \<up>(rbt_of res_t = rbt_insert k v (rbt_of t)) **
+      \<up>(rbt_sorted (rbt_of res_t)) **
+      \<up>(ptr_of_key t ti \<subseteq>\<^sub>m ptr_of_key res_t res_ti)
+    )
+  "
+  unfolding insert_opt_def rbt_insert_def rbt_insert_with_key_def paint_def
+  supply insert'_opt_correct_ext[vcg_rules]
+  apply vcg_step
+  apply vcg_step
+  apply vcg_step
+  apply vcg_step
+  apply vcg_rl
+   apply vcg_solve
+  apply vcg_solve (*where did \<up>rbt_sorted (rbt_of x) go?*)
+  apply vcg
+  apply (cases "rbt_ins (\<lambda>_ _ v. v) k v (rbt_of t)")
+  subgoal using rbt_ins_non_empty by fast
+  apply vcg
+  apply (subgoal_tac "rbt_sorted (rbt_of (ATBranch color.B x23 x24 1 li ki vi ri al ar))")
+   apply vcg_compat 
+   apply (sepEwith ignore | simp)+
+  subgoal supply ptr_of_key_subsetD[dest!] by auto
+  subgoal using ins_rbt_sorted rbt_of.simps(2) rbt_sorted.simps(2) by metis
+  done
+
+end
+
+end
