LLVM_DS_RBT/Load_Store.thy
@@ -1,0 +1,164 @@
+theory Load_Store
+  imports 
+    Assertion_Tree_Lookup
+    Extended_Assertion_Exceptions
+begin
+
+context rbt_impl
+begin
+interpretation rbt_impl_deps .
+
+subsection \<open>Load\<close>
+
+definition "load p \<equiv> do { n \<leftarrow> ll_load p; return rbt_node.val n }"
+
+lemma rbt_ptr_load_correct [vcg_rules]:
+  assumes
+    "rbt_sorted (rbt_of t)" and
+    "(kn, VALUE_EX) \<notin> ex" and
+    "(kn, PTO_EX) \<notin> ex"
+  shows
+    "
+    llvm_htriple
+    (rbt_assn_ext t ex ti ** \<up>(ptr_of_key t ti kn = Some p))
+    (load p)
+    (\<lambda>res_v.
+        \<upharpoonleft>value_assn (the (rbt_lookup (rbt_of t) kn)) res_v **
+        rbt_assn_ext t ({(kn, VALUE_EX)} \<union> ex) ti **
+        \<up>(Some res_v = value_of_key t ti kn)
+    )
+    "
+  using assms
+proof(induction t arbitrary: ti)
+  case ATEmpty 
+  show ?case by (simp add: ptr_of_key.simps)
+next
+  case (ATBranch c k v ci li ki vi ri al ar)
+  note ATBranch(1-2)[vcg_rules]
+
+  note value_of_key.simps[simp]
+
+  show ?case
+  proof(cases kn k rule: linorder_cases)
+    case less
+    moreover from less ATBranch have "kn \<guillemotleft>| rbt_of ar" by (auto intro: rbt_greater_trans)
+    moreover from less have "k \<noteq> kn" by blast
+
+    ultimately show ?thesis using ATBranch(3-5)
+      supply ptr_of_key.simps[simp]      
+      apply vcg
+      done
+  next
+    case equal
+    with ATBranch(3-5) show ?thesis
+      unfolding load_def
+      supply ptr_of_key.simps[simp]
+      apply vcg
+      unfolding rbt_assn_ext_unfold
+      apply vcg
+      done
+  next
+    case greater
+    moreover from greater ATBranch have "rbt_of al |\<guillemotleft> kn" by (auto intro: rbt_less_trans)
+    moreover from greater have "k \<noteq> kn" by blast
+
+    ultimately show ?thesis using ATBranch(3-5)
+      supply ptr_of_key.simps[simp]
+      apply vcg
+      apply simp
+      apply vcg
+      done
+  qed
+qed
+
+subsection \<open>Store\<close>
+
+definition store :: "('ki, 'vi) rbti \<Rightarrow> 'vi \<Rightarrow> unit llM" where
+  "store p v = set_value_p v p"
+
+lemma store_correct [vcg_rules]:
+  assumes
+    "rbt_sorted (rbt_of t)" and
+    "(kn, VALUE_EX) \<in> ex" and
+    "(kn, PTO_EX) \<notin> ex" and
+    "ptr_of_key t ti kn = Some p"
+  shows
+    "
+    llvm_htriple
+    (rbt_assn_ext t ex ti)
+    (store p vni)
+    (\<lambda>_. EXS res_t.
+      rbt_assn_ext res_t ex ti **
+      \<up>(rbt_of res_t = rbt_of t) **
+      \<up>(ptr_of_key res_t ti = ptr_of_key t ti) **
+      \<up>(value_of_key res_t ti = (value_of_key t ti)(kn \<mapsto> vni))
+    )
+    "
+  using assms
+proof(induction t arbitrary: ti)
+  case ATEmpty thus ?case by (simp add: ptr_of_key.simps)
+next
+  case (ATBranch c k v ci li ki vi ri l r)
+  show ?case
+  proof(cases k kn rule: linorder_cases)
+    case less
+    note ATBranch(2)[vcg_rules]
+    from less ATBranch(6) have "ptr_of_key r ri kn = Some p"
+      by (simp add: order_less_not_sym ptr_of_key.simps)
+    with less ATBranch(3-5) show ?thesis
+      apply vcg
+      apply vcg_compat
+      apply (sepEwith ignore)
+
+      subgoal by blast
+
+      subgoal for x
+        apply (rule ext)
+        unfolding ptr_of_key.simps
+        by (auto, metis)
+
+      apply (rule ext)
+      subgoal for asf sa x xa
+        apply (drule fun_cong[where x = xa])+
+        apply (auto simp add: value_of_key.simps)
+        done
+      done
+  next
+    case equal
+    with ATBranch(6) have "p = ti" by (simp add: ptr_of_key.simps) 
+    with ATBranch(3-5) equal show ?thesis
+      unfolding store_def
+      unfolding rbt_assn_ext_unfold
+      apply vcg
+      apply vcg_compat
+      apply (sepEwith \<open>auto simp add: value_of_key.simps\<close>)
+      done
+  next
+    case greater
+    note ATBranch(1)[vcg_rules]
+    from greater ATBranch(6) have "Some p = ptr_of_key l li kn"
+      by (auto simp add: ptr_of_key.simps)
+    with greater ATBranch(3-5) show ?thesis
+      apply vcg
+      apply vcg_compat
+      apply (sepEwith ignore)
+
+      subgoal by blast
+
+      subgoal for x
+        apply (rule ext)
+        unfolding ptr_of_key.simps
+        by (auto, metis)
+
+      apply (rule ext)
+      subgoal for asf sa x xa
+        apply (drule fun_cong[where x = xa])+
+        apply (auto simp add: value_of_key.simps)
+        done
+      done
+  qed
+qed
+
+end
+
+end
