LLVM_DS_RBT/Load_Store_Example.thy
@@ -1,0 +1,56 @@
+theory Load_Store_Example
+  imports 
+    Extended_Assertion
+    Utilities_Extended_Assertion
+    Assertion_Tree_Lookup
+    Lookup_Extended_Assertion
+    "Insert/Alloc_Optimized/Insert_Opt_Ext"
+    Extended_Assertion_Exceptions
+    Load_Store
+begin
+
+context rbt_impl
+begin
+interpretation rbt_impl_deps .
+
+definition "example t k1 v1 k2 v2 \<equiv>
+  do {
+    p \<leftarrow> lookup_ptr t k1;
+    t' \<leftarrow> insert_opt k2 v2 t;
+    vp \<leftarrow> load p;
+    store p v1;
+    return t'
+  }
+"
+
+lemma example_correct:
+  " rbt_sorted (rbt_of t) \<Longrightarrow> rbt_lookup (rbt_of t) k1 \<noteq> None \<Longrightarrow>
+  llvm_htriple
+  (
+    rbt_assn_ext t {} ti **
+    \<upharpoonleft>key_assn k1 k1i **
+    \<upharpoonleft>key_assn k2 k2i **
+    \<upharpoonleft>value_assn v1 v1i **
+    \<upharpoonleft>value_assn v2 v2i
+  )
+  (example ti k1i v1i k2i v2i)
+  (\<lambda>res_ti. EXS res_t res_vi res_v.
+    rbt_assn_ext res_t {} res_ti **
+    \<upharpoonleft>value_assn res_v res_vi ** \<upharpoonleft>key_assn k1 k1i **
+    \<up>(rbt_of res_t = (rbt_update (rbt_insert k2 v2 (rbt_of t)) k1 v1))
+  )
+  "
+  unfolding example_def
+  supply map_leD[elim]
+  apply vcg
+     apply auto[3]
+  apply vcg
+  apply vcg_compat
+  apply (isep_drule drule: value_ex_join_ent, (auto)[3])
+  apply simp
+  apply sepE
+  done
+
+end
+
+end
