LLVM_DS_RBT/Lookup/Lookup_Extended_Assertion.thy
@@ -1,0 +1,100 @@
+theory Lookup_Extended_Assertion
+  imports 
+    Lookup
+    "../Extended_Assertion"
+    "../Assertion_Tree_Lookup"
+begin
+
+context rbt_impl
+begin
+
+interpretation v_option: option_impl value_assn .
+
+lemma lookup_correct_ext [vcg_rules]:
+  assumes
+    copy_rule [vcg_rules]:
+    "\<And>v vi.
+      llvm_htriple
+      (\<upharpoonleft>value_assn v vi)
+      (value_copy vi)
+      (\<lambda>r. \<upharpoonleft>value_assn v vi ** \<upharpoonleft>value_assn v r)
+    "
+  shows
+    "
+      llvm_htriple
+      (rbt_assn_ext t {} ti ** \<upharpoonleft>key_assn kn ki)
+      (lookup value_copy ti ki)
+      (\<lambda>opt.
+        \<upharpoonleft>value_option_assn (rbt_lookup (rbt_of t) kn) opt **
+        rbt_assn_ext t {} ti **
+        \<upharpoonleft>key_assn kn ki)
+    "
+proof(induction t arbitrary: ti)
+  case ATEmpty
+  then show ?case
+    unfolding value_option_assn_def
+    apply (subst lookup.simps)
+    apply vcg
+    done
+next
+  case (ATBranch c l k v r)
+
+  note [vcg_rules] = ATBranch.IH
+
+  from ATBranch show ?case
+    apply (subst lookup.simps)
+    apply vcg
+    unfolding value_option_assn_def
+    apply vcg
+    done
+qed
+
+lemma lookup_ptr_corrext_ext [vcg_rules]:
+  "
+    rbt_sorted (rbt_of t) \<Longrightarrow>
+    llvm_htriple
+    (rbt_assn_ext t {} ti ** \<upharpoonleft>key_assn kn ki)
+    (lookup_ptr ti ki)
+    (\<lambda>ptr. rbt_assn_ext t {} ti ** \<upharpoonleft>key_assn kn ki **
+      \<up>(case rbt_lookup (rbt_of t) kn of None \<Rightarrow> ptr = null | _ \<Rightarrow> ptr_of_key t ti kn = Some ptr))
+  "
+proof(induction t arbitrary: ti)
+  case ATEmpty
+  then show ?case 
+    apply(subst lookup_ptr.simps)
+    apply vcg
+    done
+next
+  case (ATBranch c k v ci li ki vi ri al ar)
+  
+  note ATBranch[vcg_rules]
+
+  from ATBranch(3) show ?case
+    apply(subst lookup_ptr.simps)
+    apply vcg
+    subgoal
+      apply vcg_compat
+      apply (sep | simp?,ignore)+
+      apply (cases "rbt_lookup (rbt_of al) kn")
+      apply (auto simp add: ptr_of_key.simps)
+      done
+
+    apply vcg
+    subgoal
+      apply vcg_compat
+      apply (sep | simp?,ignore)+
+      apply (cases "rbt_lookup (rbt_of ar) kn")
+      apply (auto simp add: ptr_of_key.simps)
+      done
+
+    apply vcg
+    subgoal
+      apply vcg_compat
+      apply (sep | simp add: ptr_of_key.simps)+
+      done
+    done
+qed
+
+end
+
+end
