LLVM_DS_RBT/Separation_Logic_Solver/Append.thy
@@ -1,0 +1,20 @@
+theory Append
+  imports 
+    Main
+    "HOL-Eisbach.Eisbach_Tools"
+begin
+
+method_setup append = \<open>
+  let 
+    fun APPEND_LIST tacs = fold_rev (curry (op APPEND)) tacs (no_tac);
+  in
+   Scan.repeat1 Method.text_closure >>
+   (fn ms => fn ctxt => fn facts => let
+      val tacs = map (fn m => method_evaluate m ctxt facts) ms
+    in
+      SIMPLE_METHOD (APPEND_LIST tacs) facts
+    end)
+  end
+\<close>
+
+end
