LLVM_DS_RBT/Utilities_Extended_Assertion.thy
@@ -1,0 +1,60 @@
+theory Utilities_Extended_Assertion
+  imports 
+    Utilities
+    Extended_Assertion
+begin 
+
+context rbt_impl
+begin
+
+declare ll_matches_rbt.simps[simp]
+
+lemma matches_rbt_correct [vcg_rules]:
+  "
+  llvm_htriple
+  (rbt_assn_ext t {} ti)
+  (ll_matches_rbt pat ti)
+  (\<lambda>r. rbt_assn_ext t {} ti ** \<upharpoonleft>bool.assn (matches_rbt pat (rbt_of t)) r)
+"
+proof(induction pat arbitrary: t ti)
+  case RP_Var
+  then show ?case
+    apply vcg
+    apply (subst Hack_1) (*!FIX!*)
+    apply vcg
+    done
+next
+  case RP_Empty
+  then show ?case
+    apply vcg
+    apply (subst Hack_1) (*!FIX!*)
+    apply vcg_compat
+    apply isep_extract_pure
+    apply (simp add: bool_assn_pure_eq)
+    apply (sepwith \<open>auto elim: rbt_of.elims\<close>)+
+    done
+next
+  case (RP_Branch x1 pat1 pat2)
+  note [vcg_rules] = RP_Branch
+
+  show "?case"
+    apply vcg
+    subgoal
+      apply (subst Hack_1) (*!FIX!*)
+      apply (simp add: bool_assn_pure_eq)
+      apply vcg
+      done
+    subgoal
+      supply load_rbt_non_null[vcg_rules]
+      apply vcg
+        apply (all \<open>subst Hack_1\<close>)
+        apply vcg
+      done
+    done
+qed
+
+declare ll_matches_rbt.simps[simp del]
+
+end
+
+end
